Back to the original idea:
In the Execute method we actually allow bulk execution from our last
executed Sequence ID up to as much as we have committed sequentially
after it.

docs/sbft-formal-model/replica.i.dfy
@@ -342,13 +342,13 @@ module Replica {
                      :: v.workingWindow.committedClientOperations[seqID].Some?)
   }
 
-  predicate Execute(c:Constants, v:Variables, v':Variables, msgOps:Network.MessageOps<Message>)
+  predicate Execute(c:Constants, v:Variables, v':Variables, msgOps:Network.MessageOps<Message>, seqID:SequenceID)
   {
     && v.WF(c)
     && msgOps.NoSendRecv()
-    && var nextExecutedSeqID := v.countExecutedSeqIDs + 1;
-    && v.workingWindow.committedClientOperations[nextExecutedSeqID].Some?
-    && v' == v.(countExecutedSeqIDs := nextExecutedSeqID)
+    && v.countExecutedSeqIDs < seqID
+    && ContiguousCommits(c, v, seqID)
+    && v' == v.(countExecutedSeqIDs := seqID)
   }
 
   predicate QuorumOfPrepares(c:Constants, v:Variables, seqID:SequenceID)
@@ -514,7 +514,7 @@ module Replica {
     | SendCommitStep(seqID:SequenceID)
     | RecvCommitStep()
     | DoCommitStep(seqID:SequenceID)
-    | ExecuteStep()
+    | ExecuteStep(seqID:SequenceID)
     //| SendReplyToClient(seqID:SequenceID)
     // TODO: uncomment those steps when we start working on the proof
     // | LeaveViewStep(newView:ViewNum)
@@ -533,7 +533,7 @@ module Replica {
        case SendCommitStep(seqID) => SendCommit(c, v, v', msgOps, seqID)
        case RecvCommitStep() => RecvCommit(c, v, v', msgOps)
        case DoCommitStep(seqID) => DoCommit(c, v, v', msgOps, seqID)
-       case ExecuteStep() => Execute(c, v, v', msgOps)
+       case ExecuteStep(seqID) => Execute(c, v, v', msgOps, seqID)
        // TODO: uncomment those steps when we start working on the proof
        // case LeaveViewStep(newView) => LeaveView(c, v, v', msgOps, newView)
        // case SendViewChangeMsgStep() => SendViewChangeMsg(c, v, v', msgOps)
